list.foldl

Cm/Pi/List.lean
@@ -183,20 +183,30 @@ def list.foldl.my_f : Expr := :: π (:: id nil)
   then maps over (:: match_args (:: x xs))
 -/
 def list.foldl.mk_succ_handler :=
-  (:: both (:: (quote both) (:: both (::
-    (quote (quote apply))
+  (:: both (:: (q' both) (:: both (::
+    (q' q' apply)
   (:: both (::
-    (quote both) (:: both (::
-    ((quote const) b' list.foldl.my_f)
-    (quote (list.foldl.rec_with.get_head b' list.rec_with.advance_tail))))))))))
+    (q' both) (:: both (::
+    ((q' const) b' list.foldl.my_f)
+    (q' (list.foldl.rec_with.get_head b' list.rec_with.advance_tail))))))))))
 
 example : try_step_n' 100 (:: apply (:: (:: apply (:: list.foldl.mk_nil_handler (:: (symbol "my_f") (symbol "my_init")))) list.rec_with.test_match_args)) = (.ok (symbol "my_init")) := rfl
 
-#eval try_step_n 100 (:: apply (:: (:: apply (:: list.foldl.mk_succ_handler (:: (symbol "my_f") (symbol "my_init"))))
-  list.rec_with.test_match_args))
+example : try_step_n' 100 (:: apply (:: (:: apply (:: list.foldl.mk_succ_handler (:: (symbol "my_f") (symbol "my_init"))))
+  list.rec_with.test_match_args)) = (.ok (:: apply
+  (:: (symbol "my_f")
+     (:: (symbol "x")
+        (:: apply
+           (:: (:: apply
+                 (:: (symbol "rec_with") (:: (symbol "rec_with") (:: (symbol "nil_case") (symbol "succ_case")))))
+              (symbol "xs"))))))) := rfl
 
 def list.foldl : Expr :=
-  sorry
+  (:: both
+    (:: (quote apply) (:: both
+    (:: (quote list.rec_with) (:: both
+      (:: (quote list.rec_with)
+      (:: both (:: list.foldl.mk_nil_handler list.foldl.mk_succ_handler))))))))
 
 /-
 (:: apply (:: list.map (:: f l)))
